# Question Paper 1-3

Paper 1 for Further Maths (9231), Oct/Nov 2024, tested on ChatGPT-4o vs DeepSeek R1

## Question 4a

Use the method of differences to find (summation of 1 to n, of the following equation)((5k)/((5r+k)(5r+5+k))) in terms of n and k where k is a positive constant.

### Prompt

Use the method of differences to find (summation of 1 to n, of the following equation)((5k)/((5r+k)(5r+5+k))) in terms of n and k where k is a positive constant.

### ChatGPT Answer

We are asked to evaluate the sum:

S_n = sum from k=1 to n of (5k) / ((5r + k)(5r + 5 + k))

where k is a positive constant and r is a fixed parameter.

Step 1: Partial Fraction Decomposition
We want to decompose the general term into partial fractions. We want to express:

(5k) / ((5r + k)(5r + 5 + k)) = A / (5r + k) + B / (5r + 5 + k)

Multiply both sides of the equation by (5r + k)(5r + 5 + k) to eliminate the denominators:

5k = A(5r + 5 + k) + B(5r + k)

Now, expand both sides:

5k = A(5r + 5 + k) + B(5r + k)

5k = A(5r + 5) + A(k) + B(5r) + B(k)

5k = A(5r + 5) + B(5r) + (A + B)k

We now compare the coefficients of like powers of k:

The coefficient of k on the left-hand side is 5, so we have:
A + B = 5

The constant term on the left-hand side is 0 (since there is no constant term on the left side), so we have:
A(5r + 5) + B(5r) = 0

Step 2: Solve for A and B
From the equation A + B = 5, we can express B as:

B = 5 - A

Substitute B = 5 - A into the second equation A(5r + 5) + B(5r) = 0:

A(5r + 5) + (5 - A)(5r) = 0

Expanding:

A(5r + 5) + 5(5r) - A(5r) = 0

Simplify the terms:

A(5r + 5) + 25r - A(5r) = 0

A(5r + 5 - 5r) = -25r

A(5) = -25r

A = -5r

Now, substitute A = -5r into B = 5 - A:

B = 5 - (-5r) = 5 + 5r

Step 3: Substitute A and B Back
Now that we have A = -5r and B = 5 + 5r, we can rewrite the general term:

(5k) / ((5r + k)(5r + 5 + k)) = (-5r) / (5r + k) + (5 + 5r) / (5r + 5 + k)

Step 4: Express the Sum
Now we can express the sum as:

S_n = sum from k=1 to n of [ (-5r) / (5r + k) + (5 + 5r) / (5r + 5 + k) ]

This sum is now split into two simpler sums:

S_n = -5r * sum from k=1 to n of [ 1 / (5r + k) ] + (5 + 5r) * sum from k=1 to n of [ 1 / (5r + 5 + k) ]

Step 5: Simplify the Sums
Now, observe that these are both standard summations, where we are summing fractions of the form 1 / (5r + k). The first sum starts at k = 1, and the second sum starts at k = 6. These sums are standard sums of reciprocals of linear terms.

Thus, the full expression for the sum S_n is:

S_n = -5r * sum from k=1 to n of [ 1 / (5r + k) ] + (5 + 5r) * sum from k=1 to n of [ 1 / (5r + 5 + k) ]

This is the final expression for the sum in terms of n and r, using the method of differences. The sums themselves are standard harmonic sums, which can be evaluated numerically for specific values of n and r.

### DeepSeek Thinking

Okay, so I need to find the sum from r = 1 to n of (5k) divided by (5r + k)(5r + 5 + k). The question says to use the method of differences, which I remember is also called telescoping. The idea is to break the term into a difference of two fractions so that when you add them up, most terms cancel out. Let me see how to apply that here.

First, the general term is (5k)/[(5r + k)(5r + 5 + k)]. Let me denote this as T_r. So,

T_r = 5k / [(5r + k)(5r + 5 + k)]

I need to express this as a difference of two fractions. Let's assume that T_r can be written as A/(5r + k) - B/(5r + 5 + k), where A and B are constants to be determined. If this is possible, then when we sum over r from 1 to n, most terms will cancel, leaving only the first and last terms.

So, let's set up the equation:

5k / [(5r + k)(5r + 5 + k)] = A/(5r + k) - B/(5r + 5 + k)

To find A and B, let's combine the right-hand side over a common denominator:

[A(5r + 5 + k) - B(5r + k)] / [(5r + k)(5r + 5 + k)] = 5k / [(5r + k)(5r + 5 + k)]

Since the denominators are the same, the numerators must be equal:

A(5r + 5 + k) - B(5r + k) = 5k

Let's expand the left-hand side:

A*5r + A*(5 + k) - B*5r - B*k = 5k

Now, group the terms with r and the constant terms:

(5A - 5B)r + [A(5 + k) - Bk] = 5k

Since this must hold for all values of r, the coefficients of r and the constant term must each be equal on both sides. On the right-hand side, the coefficient of r is 0, and the constant term is 5k.

Therefore, we have two equations:

1. Coefficient of r: 5A - 5B = 0

2. Constant term: A(5 + k) - Bk = 5k

From the first equation, 5A - 5B = 0 ⇒ A = B

Substitute A = B into the second equation:

A(5 + k) - A*k = 5k

Simplify:

A*5 + A*k - A*k = 5k ⇒ 5A = 5k ⇒ A = k

Since A = B, then B = k as well.

So, the original term T_r can be written as:

T_r = k/(5r + k) - k/(5r + 5 + k)

Therefore, the sum from r = 1 to n of T_r is:

Sum = Σ_{r=1}^n [k/(5r + k) - k/(5(r + 1) + k)]

Notice that in the second term, 5r + 5 + k can be written as 5(r + 1) + k. So, when we write out the terms, we get:

For r = 1: k/(5*1 + k) - k/(5*2 + k)

For r = 2: k/(5*2 + k) - k/(5*3 + k)

...

For r = n: k/(5n + k) - k/(5(n + 1) + k)

When we add all these up, the intermediate terms cancel out. The -k/(5*2 + k) from the first term cancels with the +k/(5*2 + k) from the second term, and so on. This telescoping effect continues until all that remains is the first term of the first expression and the second term of the last expression.

Therefore, the sum simplifies to:

Sum = [k/(5*1 + k) - k/(5(n + 1) + k)]

Simplify each term:

First term: k/(5 + k)

Second term: k/(5(n + 1) + k) = k/(5n + 5 + k)

Therefore, the total sum is:

Sum = k/(5 + k) - k/(5n + 5 + k)

We can factor out k:

Sum = k[1/(5 + k) - 1/(5n + 5 + k)]

To combine these fractions, find a common denominator, which is (5 + k)(5n + 5 + k):

Sum = k[(5n + 5 + k) - (5 + k)] / [(5 + k)(5n + 5 + k)]

Simplify the numerator:

(5n + 5 + k - 5 - k) = 5n

Therefore:

Sum = k*5n / [(5 + k)(5n + 5 + k)] = (5kn) / [(5 + k)(5n + 5 + k)]

We can factor 5 from the denominator's second term:

5n + 5 + k = 5(n + 1) + k

But perhaps it's better left as is. Let me check if there's a simpler form.

Alternatively, the expression is (5kn)/[(5 + k)(5(n + 1) + k)]

But the problem states to present the answer in terms of n and k, so this should be acceptable.

Wait, but let me verify my steps again to make sure I didn't make any mistakes.

Starting from the partial fractions:

T_r = 5k / [(5r + k)(5r + 5 + k)] = k/(5r + k) - k/(5r + 5 + k)

Then the sum telescopes, leaving k/(5 + k) - k/(5n + 5 + k). Then combining these gives the expression with 5kn in the numerator.

Yes, that seems correct.

Alternatively, if we want to write the final answer as a single fraction, it's (5kn)/[(5 + k)(5n + 5 + k)].

Alternatively, factor 5 from the second term in the denominator:

= (5kn)/[(5 + k)(5(n + 1) + k)]

Either form is acceptable, but perhaps the first one is simpler. Let me check with n=1 to see if it matches.

For n=1, the original sum is just the term when r=1:

5k / [(5*1 + k)(5*1 + 5 + k)] = 5k / [(5 + k)(10 + k)]

Using the formula:

(5k*1)/[(5 + k)(5*1 + 5 + k)] = 5k / [(5 + k)(10 + k)] which matches. So that's correct.

Another test: n=2. The sum should be the sum of r=1 and r=2 terms.

First term: 5k / [(5 + k)(10 + k)]

Second term: 5k / [(10 + k)(15 + k)]

Total sum: 5k/(5 + k)(10 + k) + 5k/(10 + k)(15 + k) = 5k/(10 + k)[1/(5 + k) + 1/(15 + k)]

Using the formula:

(5k*2)/[(5 + k)(5*2 + 5 + k)] = 10k / [(5 + k)(15 + k)]

Comparing with the sum:

5k/(10 + k)[1/(5 + k) + 1/(15 + k)] = 5k/(10 + k)[ (15 + k + 5 + k) / ( (5 + k)(15 + k) ) ] = 5k/(10 + k)[ (20 + 2k) / ( (5 + k)(15 + k) ) ] = (5k*(20 + 2k)) / [ (10 + k)(5 + k)(15 + k) ) ]

Wait, but according to the formula, it's 10k / [ (5 + k)(15 + k) )

So, unless 5k*(20 + 2k) / [ (10 + k)(5 + k)(15 + k) ) ] = 10k / [ (5 + k)(15 + k) )

Simplify left side: [5k*(20 + 2k)] / [ (10 + k)(5 + k)(15 + k) ) ] = [10k*(10 + k)] / [ (10 + k)(5 + k)(15 + k) ) ] = 10k / [ (5 + k)(15 + k) ) ]

Yes! Because 5k*(20 + 2k) = 5k*2*(10 + k) = 10k*(10 + k). So numerator and denominator have (10 + k) cancels out. Thus, left side equals 10k / [ (5 + k)(15 + k) ), which matches the formula. Therefore, the formula works for n=2. So, that seems correct.

Hence, the answer is Sum = (5kn)/[(5 + k)(5n + 5 + k)]

Alternatively, written as:

Sum = (5kn) / [ (5 + k)(5(n + 1) + k) ]

Either way is correct, but I'll present it as:

Sum = \frac{5kn}{(5 + k)(5n + 5 + k)}

Alternatively, factor 5 from the denominator's second term:

Sum = \frac{5kn}{(5 + k)(5(n + 1) + k)}

Either form is acceptable. Since the problem says "in terms of n and k", both forms are correct. But perhaps the first form is preferable as it directly shows 5n +5 +k.

But let me check again. If we write 5n +5 +k =5(n +1) +k, which might be a bit more factored. Maybe that's better. But unless specified, both are correct.

Alternatively, the problem may want the answer simplified as much as possible. Let me check the numerator and denominator for common factors. The numerator is 5kn, denominator is (5 +k)(5n +5 +k). There's a 5 in the numerator and 5 in the denominator's second term. Let's see:

Factor 5 from the denominator's second term:

(5(n +1) +k). So denominator is (5 +k)(5(n +1) +k). The numerator is 5kn.

So we can write:

5kn / [ (5 +k)(5(n +1) +k) ] = [5/(5 +k)] * [ kn / (5(n +1) +k) ]

But that doesn't really simplify further. So maybe the original expression is the simplest.

Alternatively, if we factor 5 from both numerator and denominator:

But denominator is (5 +k)(5(n +1) +k). There's a 5 in the second bracket. The numerator is 5kn. So we can write:

5kn / [ (5 +k)(5(n +1) +k) ] = kn / [ (5 +k)(n +1 + k/5) ]

But this might not be necessary. The problem doesn't specify the form, so probably either is acceptable. However, to present it as per telescoping sum result, perhaps writing it as:

Sum = \frac{k}{5 + k} - \frac{k}{5(n +1) + k}

But the question says to present it in terms of n and k, so they might prefer the combined fraction. Let me check the problem statement again: "find (summation of 1 to n, of the following equation)((5k)/((5r+k)(5r+5+k))) in terms of n and k where k is a positive constant."

So the answer should be expressed as a single expression in terms of n and k. So the telescoped form is two terms, but combining them gives the single fraction. Hence, the combined form is better.

Thus, the answer is:

Sum = \frac{5kn}{(5 + k)(5n + 5 + k)}

Alternatively, written as:

Sum = \frac{5kn}{(5 + k)(5(n + 1) + k)}

Either is correct. To confirm, let's compute for k=5, n=1. If k=5, then the term is (25)/[(5r +5)(5r +10)] =25/[5(r +1)*5(r +2)] =25/[25(r +1)(r +2)] =1/[(r +1)(r +2)]

So the sum from r=1 to n=1 would be 1/(2*3)=1/6.

Using the formula:

5kn/( (5 +k)(5n +5 +k) )=5*5*1/( (10)(5*1 +5 +5))=25/(10*15)=25/150=1/6. Correct.

Another check with k=0. Wait, but k is a positive constant, so k=0 is not allowed. Let's try k=1, n=2.

Original sum: for r=1, 5*1 / (5 +1)(10 +1) =5/(6*11)=5/66

For r=2, 5*1 / (10 +1)(15 +1)=5/(11*16)=5/176

Total sum:5/66 +5/176= (5*176 +5*66)/(66*176)=5(176 +66)/66*176=5*242/(66*176)=1210/(11616). Simplify:

Divide numerator and denominator by 2:605/5808. Divide by 11:55/528. Divide by 11 again:5/48. Wait, 55 divided by 11 is 5, 528 divided by 11 is 48. So 5/48.

Using the formula:

5kn/( (5 +k)(5n +5 +k) )=5*1*2/(6*15 +1*2? Wait, wait. Wait k=1, n=2.

Wait denominator is (5 +k)(5n +5 +k). So (5 +1)=6, (5*2 +5 +1)=10 +5 +1=16. So denominator=6*16=96.

Numerator=5*1*2=10. So 10/96=5/48. Which matches the manual calculation. Perfect.

So the formula works. Therefore, the answer is correct.

The summation is equal to \boxed{\dfrac{5kn}{(5 + k)(5n + 5 + k)}}.

### DeepSeek Answer

To find the sum from r equals 1 to n of (5k) divided by (5r + k)(5r + 5 + k) using the method of differences:

Rewrite the term as a telescoping series:
Term_r = [k divided by (5r + k)] minus [k divided by (5(r + 1) + k)].

Sum Term_r from r = 1 to n:
Total = [k divided by (51 + k) minus k divided by (52 + k)] +
[k divided by (52 + k) minus k divided by (53 + k)] + ... +
[k divided by (5n + k) minus k divided by (5(n+1) + k)].

Most terms cancel. Only the first and last remain:
Total = k divided by (5 + k) minus k divided by (5(n + 1) + k).

Final result:
k divided by (5 + k) minus k divided by (5n + 5 + k).

### Verdict

ChatGPT 0, DeepSeek 4

ChatGPT made an error in the algebra for the telescoping summation, while DeepSeek solved it correctly and found the right answer.

Total Marks so far: ChatGPT 14, DeepSeek 31

## Question 4b

It is given that the sum to infinity is 1/3.

Find the value of k. 

### Prompt

It is given that the sum to infinity is 1/3.

Find the value of k. 

### ChatGPT Answer

Can't solve because of the mistake in the 4a.

### DeepSeek Answer

Here is the step-by-step solution in plain text:

Infinite Sum Expression:
From the earlier result, the sum to infinity is the limit as n approaches infinity of:
[k divided by (5 + k)] minus [k divided by (5(n + 1) + k)].

As n becomes very large, the term [k divided by (5(n + 1) + k)] becomes zero.
So the infinite sum simplifies to:
k divided by (5 + k).

Set the Sum Equal to 1/3:
k divided by (5 + k) = 1/3.

Solve for k:
Multiply both sides by (5 + k):
3k = 5 + k.
Subtract k from both sides:
2k = 5.
Divide by 2:
k = 5/2 (or 2.5).

Final Answer:
k = 5/2.

### Verdict

ChatGPT 0, DeepSeek 2

Total Marks so far: ChatGPT 14, DeepSeek 33

## Question 4c

Hence find summation from n to n^2 of (5k)/((5r+k)(5r+5+k)) in terms of n.

### Prompt

Hence find summation from n to n^2 of (5k)/((5r+k)(5r+5+k)) in terms of n.

### ChatGPT Answer

Can't solve because it did not solve 4a or 4b.

### DeepSeek Thinking

Okay, let me try to figure out how to find the summation from n to n² of the term (5k)/[(5r + k)(5r + 5 + k)] in terms of n. First, I remember from the previous problem that when we summed from r = 1 to n, we ended up with a telescoping series that simplified nicely. The result was k/(5 + k) - k/(5(n + 1) + k). Now, the user is asking to sum from r = n to r = n² instead of from 1 to n.

Wait, so maybe I can use the same telescoping approach but adjust the limits of summation. Let me recall how telescoping series work. The key idea is that consecutive terms cancel out, leaving only the first and last terms. So if I can express the general term as a difference of two fractions, the sum should collapse to the difference between the first term of the first expression and the last term of the second expression.

In the original problem, the term was decomposed into [k/(5r + k)] - [k/(5(r + 1) + k)]. If I sum this from r = a to r = b, the sum should be [k/(5a + k)] - [k/(5(b + 1) + k)]. Applying this to the current problem where the summation is from r = n to r = n², the sum should be [k/(5n + k)] - [k/(5(n² + 1) + k)].

But wait, let me verify this. Let's substitute a = n and b = n². Then the sum from r = a to b of [k/(5r + k) - k/(5(r + 1) + k)] would indeed be the first term at r = a minus the last term at r = b + 1. So yes, it would be [k/(5n + k)] - [k/(5(n² + 1) + k)].

But hold on, the original summation was from r = 1 to n, and we had k/(5 + k) - k/(5(n + 1) + k). Here, starting at r = n, the first term in the telescoping sum would be k/(5n + k), and the last term would be k/(5(n² + 1) + k). Therefore, the total summation should be the difference between these two terms.

However, I need to make sure that there are no miscalculations here. Let me test with a small value of n. Suppose n = 2. Then the summation from r = 2 to r = 4 (since n² = 4) would be three terms: r = 2, 3, 4. Each term is [k/(5r + k)] - [k/(5(r + 1) + k)]. So:

For r = 2: [k/(10 + k)] - [k/(15 + k)]

For r = 3: [k/(15 + k)] - [k/(20 + k)]

For r = 4: [k/(20 + k)] - [k/(25 + k)]

Adding these up: [k/(10 + k) - k/(15 + k)] + [k/(15 + k) - k/(20 + k)] + [k/(20 + k) - k/(25 + k)] = k/(10 + k) - k/(25 + k).

Which matches the formula [k/(5n + k)] - [k/(5(n² + 1) + k)] when n = 2: [k/(10 + k)] - [k/(25 + k)]. So the formula works here. Therefore, the general formula for the summation from r = n to r = n² is indeed [k/(5n + k)] - [k/(5(n² + 1) + k)].

But the problem says to express the summation in terms of n. Since k was previously found to be 5/2 for the infinite sum to be 1/3, but here the problem doesn't specify to use that k. Wait, the problem says "Hence find summation from n to n² of (5k)/((5r+k)(5r+5+k)) in terms of n." The "Hence" suggests that we should use the previous result where k was determined. But in the previous step, k was found to be 5/2 when the infinite sum equals 1/3. However, this problem doesn't mention the infinite sum; it's a separate question. Wait, maybe the problem is part of the same sequence where k was found to be 5/2, so perhaps we need to substitute k = 5/2 into the summation formula.

But the user hasn't specified whether k is still 5/2 here. Let me check the original problem statement. The original problem was to find the summation in terms of n and k where k is a positive constant. Then in a subsequent problem, given that the sum to infinity is 1/3, k was found to be 5/2. Now, the current problem says "Hence find summation from n to n²..." which suggests that this is a follow-up to the previous question where k was determined. Therefore, likely substituting k = 5/2 into the summation formula.

But the problem says "in terms of n" which might imply that k is still a variable. Wait, the original problem didn't specify k being a particular value until the sum to infinity was given. But the current problem might be separate, asking to express the sum in terms of n (with k still being a constant). However, the "Hence" suggests building on the previous step where k was found. Let me recheck.

Original problem sequence:

1. Find summation from 1 to n of (5k)/[(5r+k)(5r+5+k)] in terms of n and k.

2. Given sum to infinity is 1/3, find k (which was 5/2).

3. Hence find summation from n to n² of (5k)/[...] in terms of n.

The word "Hence" indicates that we should use the previous result, i.e., k = 5/2. Therefore, substitute k = 5/2 into the summation formula and express the result in terms of n.

But let me confirm. If we proceed with k = 5/2, then the summation from r = n to n² would be [k/(5n + k)] - [k/(5(n² + 1) + k)]. Plugging k = 5/2:

First term: (5/2)/(5n + 5/2) = (5/2)/(5n + 5/2) = (5/2)/( (10n + 5)/2 ) = 5/(10n + 5) = 1/(2n + 1)

Second term: (5/2)/(5(n² + 1) + 5/2) = (5/2)/(5n² + 5 + 5/2) = (5/2)/(5n² + 15/2) = (5/2)/( (10n² + 15)/2 ) = 5/(10n² + 15) = 1/(2n² + 3)

Therefore, the summation from n to n² would be 1/(2n + 1) - 1/(2n² + 3)

But wait, the problem says "in terms of n" and if k is given as 5/2 from the previous step, then this would be the answer. However, if the problem is still considering k as a variable, then the answer would be in terms of both k and n, but the "Hence" suggests using the found value of k. However, the problem statement isn't entirely clear. Let me check the exact wording:

"Hence find summation from n to n^2 of (5k)/((5r+k)(5r+5+k)) in terms of n."

The "Hence" likely refers to using the previous result where k was determined, so substituting k = 5/2. Thus, the answer would be in terms of n only, since k is now known as 5/2. Therefore, substituting k = 5/2 into the expression [k/(5n + k)] - [k/(5(n² + 1) + k)] gives the result in terms of n.

But let me make sure. Let's re-express the general summation from r = a to r = b:

Sum = [k/(5a + k)] - [k/(5(b + 1) + k)]

In this case, a = n and b = n², so:

Sum = [k/(5n + k)] - [k/(5(n² + 1) + k)]

If k is 5/2, substituting:

First term: (5/2)/(5n + 5/2) = (5/2)/( (10n + 5)/2 ) = 5/(10n + 5) = 1/(2n + 1)

Second term: (5/2)/(5(n² + 1) + 5/2) = (5/2)/(5n² + 5 + 5/2) = (5/2)/( (10n² + 10 + 5)/2 ) = 5/(10n² + 15) = 1/(2n² + 3)

Therefore, the summation is 1/(2n + 1) - 1/(2n² + 3)

Simplifying this expression if possible. Let's combine the fractions:

Common denominator is (2n + 1)(2n² + 3)

Numerator: (2n² + 3) - (2n + 1) = 2n² + 3 - 2n - 1 = 2n² - 2n + 2

Factor numerator: 2(n² - n + 1)

But since it's 2n² - 2n + 2 = 2(n² - n + 1). Therefore, the combined fraction is 2(n² - n + 1)/[(2n + 1)(2n² + 3)]

However, this might not simplify further, so the simplest form is likely 1/(2n + 1) - 1/(2n² + 3)

Alternatively, leaving it as the difference of two fractions is acceptable. The problem says "in terms of n," which can be expressed either way, but the telescoped form is probably preferred.

Therefore, the final answer is 1/(2n + 1) - 1/(2n² + 3), which can be written as [1/(2n + 1)] - [1/(2n² + 3)] or combined over a common denominator if required. However, since the problem asks to "find" the summation, expressing it as the telescoped difference is sufficient.

### DeepSeek Answer

To find the sum from r = n to r = n squared

Use the telescoping formula from earlier:
Sum = [k divided by (5n + k)] minus [k divided by (5(n squared + 1) + k)].

Substitute k = 5 divided by 2 (since k = 5/2 from the previous result):

First term: (5/2) divided by (5n + 5/2) = (5/2) divided by (5n + 2.5) = simplified to 1 divided by (2n + 1).

Second term: (5/2) divided by (5(n squared + 1) + 5/2) = (5/2) divided by (5n squared + 5 + 2.5) = simplified to 1 divided by (2n squared + 3).

Final result:
[1 divided by (2n + 1)] minus [1 divided by (2n squared + 3)].

Answer:
1/(2n + 1) - 1/(2n squared + 3).

### Verdict

ChatGPT 0 DeepSeek 2

Total Marks so far: ChatGPT 14, DeepSeek 35
