# Question Paper 1-3

Paper 1 for Further Maths (9231), Oct/Nov 2024, tested on ChatGPT-4o vs DeepSeek R1

## Question 6a

The curve C has equation y = (4x^2 + x + 1)/(2x^2 - 7x + 3).

Find the equations of the asymptotes of C.

### ChatGPT Answer

To find the equations of the asymptotes of the curve given by:

y = (4x^2 + x + 1) / (2x^2 - 7x + 3)

we need to consider both the vertical asymptotes (when the denominator is zero) and the oblique or horizontal asymptotes (for large values of x).

1. Vertical Asymptotes
Vertical asymptotes occur where the denominator of the function equals zero, and the numerator is non-zero at those points.

We find the vertical asymptotes by setting the denominator equal to zero:

2x^2 - 7x + 3 = 0

We can solve this quadratic equation using the quadratic formula:

x = (-(-7) ± √((-7)^2 - 4(2)(3))) / 2(2)

x = (7 ± √(49 - 24)) / 4

x = (7 ± √25) / 4

x = (7 ± 5) / 4

Thus, the two solutions are:

x = (7 + 5) / 4 = 12 / 4 = 3

x = (7 - 5) / 4 = 2 / 4 = 1/2

So, the vertical asymptotes are at:

x = 3 and x = 1/2

2. Oblique or Horizontal Asymptotes
For horizontal or oblique asymptotes, we need to examine the behavior of the function as x → ∞ or x → -∞.

Horizontal Asymptote:
If the degree of the numerator and denominator are the same, the horizontal asymptote is given by the ratio of the leading coefficients.

In this case, both the numerator and denominator are quadratic polynomials, and the leading coefficient of the numerator is 4, while the leading coefficient of the denominator is 2. Therefore, the horizontal asymptote is:

y = 4 / 2 = 2

Conclusion:
The equations of the asymptotes for the curve are:

Vertical asymptotes: x = 3 and x = 1/2
Horizontal asymptote: y = 2

### DeepSeek Answer

To find the equations of the asymptotes for the curve C given by y = (4x^2 + x + 1)/(2x^2 - 7x + 3):

Vertical Asymptotes:

Factor the denominator: 2x^2 - 7x + 3 = (2x - 1)(x - 3).

The denominator equals zero when 2x - 1 = 0 or x - 3 = 0, giving x = 1/2 and x = 3.

Check the numerator at these x-values:

At x = 1/2: Numerator = 4*(1/2)^2 + (1/2) + 1 = 1 + 0.5 + 1 = 2.5 ≠ 0.

At x = 3: Numerator = 4*(3)^2 + 3 + 1 = 36 + 3 + 1 = 40 ≠ 0.

Since the numerator is non-zero at both x = 1/2 and x = 3, these are vertical asymptotes.

Horizontal Asymptote:

The degrees of the numerator and denominator are equal (both degree 2).

The horizontal asymptote is the ratio of the leading coefficients: 4/2 = 2.

Horizontal asymptote: y = 2.

Oblique Asymptotes:

Oblique (slant) asymptotes occur when the degree of the numerator is exactly one greater than the denominator. Here, the degrees are equal, so there are no oblique asymptotes.

Holes:

Check for common factors in the numerator and denominator.

The numerator 4x^2 + x + 1 does not factor further (it has no real roots) and shares no common factors with the denominator (2x - 1)(x - 3). Thus, there are no holes.

Equations of the asymptotes:

Vertical asymptotes: x = 1/2 and x = 3

Horizontal asymptote: y = 2

Final answer:
x = 1/2, x = 3, and y = 2.

### Verdict

ChatGPT 2, DeepSeek 2

Total Marks so far: ChatGPT 23, DeepSeek 49

## Question 6b

Find the coordinates of any stationary points on C.

### ChatGPT Answer

To find the stationary points of the curve 
𝐶
C with the equation:

y = (4x² + x + 1) / (2x² - 7x + 3)

we need to find the points where the derivative of y is zero. A stationary point occurs when the derivative of y with respect to x is zero (i.e., dy/dx = 0).

Step 1: Differentiate the equation using the quotient rule
We will differentiate the function using the quotient rule, which states:

dy/dx = (v(x) * u'(x) - u(x) * v'(x)) / (v(x))²

Here, u(x) = 4x² + x + 1 and v(x) = 2x² - 7x + 3.

The derivative of u(x) = 4x² + x + 1 is:
u'(x) = 8x + 1

The derivative of v(x) = 2x² - 7x + 3 is:
v'(x) = 4x - 7

Now apply the quotient rule:

dy/dx = ((2x² - 7x + 3)(8x + 1) - (4x² + x + 1)(4x - 7)) / (2x² - 7x + 3)²

Step 2: Set the derivative equal to zero
To find the stationary points, we set dy/dx = 0, which means the numerator must equal zero. Therefore, we solve:

(2x² - 7x + 3)(8x + 1) - (4x² + x + 1)(4x - 7) = 0

We need to expand both terms and then solve the resulting equation for x.

Step 3: Expand and simplify
Expand (2x² - 7x + 3)(8x + 1):
(2x² - 7x + 3)(8x + 1) = 2x²(8x + 1) - 7x(8x + 1) + 3(8x + 1)
= 16x³ + 2x² - 56x² - 7x + 24x + 3
= 16x³ - 54x² + 17x + 3

Expand (4x² + x + 1)(4x - 7):
(4x² + x + 1)(4x - 7) = 4x²(4x - 7) + x(4x - 7) + 1(4x - 7)
= 16x³ - 28x² + 4x² - 7x + 4x - 7
= 16x³ - 24x² - 3x - 7

Step 4: Subtract the two expressions
Now, subtract the second expanded expression from the first:

(16x³ - 54x² + 17x + 3) - (16x³ - 24x² - 3x - 7)
= 16x³ - 54x² + 17x + 3 - 16x³ + 24x² + 3x + 7
= (-54x² + 24x²) + (17x + 3x) + (3 + 7)
= -30x² + 20x + 10

Thus, the numerator simplifies to:

-30x² + 20x + 10 = 0

Step 5: Solve the quadratic equation
Now, solve the quadratic equation:

-30x² + 20x + 10 = 0

Divide through by -10 to simplify:

3x² - 2x - 1 = 0

We can solve this using the quadratic formula:

x = (-(-2) ± √((-2)² - 4(3)(-1))) / 2(3)
x = (2 ± √(4 + 12)) / 6
x = (2 ± √16) / 6
x = (2 ± 4) / 6

So, the two solutions are:

x = (2 + 4) / 6 = 6 / 6 = 1
x = (2 - 4) / 6 = -2 / 6 = -1/3

Step 6: Find the corresponding y-values
Now, substitute these x-values back into the original equation for y:

For x = 1:
y = (4(1)² + 1 + 1) / (2(1)² - 7(1) + 3)
= (4 + 1 + 1) / (2 - 7 + 3)
= 6 / -2
= -3

So, one stationary point is (1, -3).

For x = -1/3:
y = (4(-1/3)² + (-1/3) + 1) / (2(-1/3)² - 7(-1/3) + 3)
= (4(1/9) - 1/3 + 1) / (2(1/9) + 7/3 + 3)
= (4/9 - 3/9 + 9/9) / (2/9 + 21/9 + 27/9)
= 10/9 / 50/9
= 10/50
= 1/5

So, the other stationary point is (-1/3, 1/5).

Conclusion:
The stationary points on the curve C are:

(1, -3)
(-1/3, 1/5)

### DeepSeek Answer

To find the coordinates of the stationary points on the curve C with equation y = (4x^2 + x + 1)/(2x^2 - 7x + 3):

Find the derivative dy/dx using the quotient rule:

Let u = 4x^2 + x + 1 and v = 2x^2 - 7x + 3.

Compute u' = 8x + 1 and v' = 4x - 7.

Apply the quotient rule

Simplify the numerator:

Expand (2x^2 - 7x + 3)(8x + 1):
= 16x^3 - 56x^2 + 24x + 2x^2 - 7x + 3
= 16x^3 - 54x^2 + 17x + 3.

Expand (4x^2 + x + 1)(4x - 7):
= 16x^3 - 28x^2 + 4x^2 - 7x + 4x - 7
= 16x^3 - 24x^2 - 3x - 7.

Subtract the second expansion from the first:
Numerator = (16x^3 - 54x^2 + 17x + 3) - (16x^3 - 24x^2 - 3x - 7)
= -30x^2 + 20x + 10.

Set dy/dx = 0 and solve for x:

Solve -30x^2 + 20x + 10 = 0:
Divide by -10: 3x^2 - 2x - 1 = 0.
Use quadratic formula: x = [2 ± sqrt(4 + 12)] / 6 = [2 ± sqrt(16)] / 6 = [2 ± 4]/6.
Solutions: x = (2 + 4)/6 = 1 or x = (2 - 4)/6 = -1/3.

Find the corresponding y-coordinates:

For x = 1:
y = [4(1)^2 + 1 + 1] / [2(1)^2 - 7(1) + 3] = (4 + 1 + 1)/(2 - 7 + 3) = 6/(-2) = -3.
Point: (1, -3).

For x = -1/3:
Compute numerator:
4(-1/3)^2 + (-1/3) + 1 = 4*(1/9) - 1/3 + 1 = 4/9 - 3/9 + 9/9 = 10/9.
Compute denominator:
2(-1/3)^2 - 7(-1/3) + 3 = 2*(1/9) + 7/3 + 3 = 2/9 + 21/9 + 27/9 = 50/9.
y = (10/9)/(50/9) = 10/50 = 1/5.
Point: (-1/3, 1/5).

Coordinates of the stationary points:
(1, -3) and (-1/3, 1/5).

### Verdict

ChatGPT 4, DeepSeek 4

Total Marks so far: ChatGPT 27, DeepSeek 53