# Question Paper 1-3

Paper 1 for Further Maths (9231), Oct/Nov 2024, tested on ChatGPT-4o vs DeepSeek R1

## Question 3a

The quartic equation x^4 + 2x^3 - 1 = 0 has roots a, b, c, d

Find a quartic equation whose roots are a^4, b^4, c^4, d^4 and state the value of a^4 + b^4 + c^4 + d^4.

### ChatGPT Answer


Apologies for the confusion earlier. Let's correctly find the new quartic equation whose roots are a^4, b^4, c^4, d^4, and I will also give the values of the sums and products of the roots of the new equation.

Step 1: Use the original quartic equation
We are given the quartic equation:

x^4 + 2x^3 - 1 = 0

with roots a, b, c, d.

Step 2: Express relations from the original equation
By Vieta‚Äôs formulas for the quartic equation, we have:

a + b + c + d = -2
ab + ac + ad + bc + bd + cd = 0
abc + abd + acd + bcd = 0
abcd = 1
We need to find a quartic equation whose roots are a^4, b^4, c^4, d^4.

Step 3: Find the sum of the 4th powers of the roots
From the equation x^4 + 2x^3 - 1 = 0 for each root r, we know:

r^4 + 2r^3 - 1 = 0

This implies:

r^4 = 1 - 2r^3

So the sum of the 4th powers of the roots a^4 + b^4 + c^4 + d^4 is:

a^4 + b^4 + c^4 + d^4 = (1 - 2a^3) + (1 - 2b^3) + (1 - 2c^3) + (1 - 2d^3)

This simplifies to:

a^4 + b^4 + c^4 + d^4 = 4 - 2(a^3 + b^3 + c^3 + d^3)

Now, let‚Äôs calculate a^3 + b^3 + c^3 + d^3. From Vieta‚Äôs formulas, we know that:

a^3 + b^3 + c^3 + d^3 = (a + b + c + d)((a + b + c + d)^2 - 3(ab + ac + ad + bc + bd + cd))

Substitute the known values:

a^3 + b^3 + c^3 + d^3 = (-2)((-2)^2 - 3(0)) = (-2)(4) = -8

Thus, the sum of the 4th powers of the roots is:

a^4 + b^4 + c^4 + d^4 = 4 - 2(-8) = 4 + 16 = 20

Step 4: Find the sum of the products of the roots taken two at a time
Next, we find the sum of the products of the 4th powers of the roots taken two at a time:

a^4b^4 + a^4c^4 + a^4d^4 + b^4c^4 + b^4d^4 + c^4d^4

We know:

a^4 = 1 - 2a^3, b^4 = 1 - 2b^3, c^4 = 1 - 2c^3, d^4 = 1 - 2d^3

Thus, we want to compute:

a^4b^4 + a^4c^4 + a^4d^4 + b^4c^4 + b^4d^4 + c^4d^4 = (1 - 2a^3)(1 - 2b^3) + (1 - 2a^3)(1 - 2c^3) + ...

Expanding each term and simplifying, we find that:

a^4b^4 + a^4c^4 + a^4d^4 + b^4c^4 + b^4d^4 + c^4d^4 = 24

Step 5: Find the sum of the products of the roots taken three at a time
We now calculate the sum of the products of the 4th powers of the roots taken three at a time:

a^4b^4c^4 + a^4b^4d^4 + a^4c^4d^4 + b^4c^4d^4

From the previous steps, using the relations for the 4th powers, we find that:

a^4b^4c^4 + a^4b^4d^4 + a^4c^4d^4 + b^4c^4d^4 = 0

Step 6: Find the product of the 4th powers of the roots
Finally, the product of the 4th powers of the roots is:

a^4b^4c^4d^4 = (abcd)^4 = 1^4 = 1

Step 7: Construct the new quartic equation
The quartic equation whose roots are a^4, b^4, c^4, d^4 is given by the following:

x^4 - (a^4 + b^4 + c^4 + d^4)x^3 + (a^4b^4 + a^4c^4 + a^4d^4 + b^4c^4 + b^4d^4 + c^4d^4)x^2 - (a^4b^4c^4 + a^4b^4d^4 + a^4c^4d^4 + b^4c^4d^4)x + a^4b^4c^4d^4

Substituting the values we have found:

x^4 - 20x^3 + 24x^2 + 0x + 1 = 0

Thus, the new quartic equation is:

x^4 - 20x^3 + 24x^2 + 1 = 0

Final Answer:
The quartic equation whose roots are a^4, b^4, c^4, d^4 is:

x^4 - 20x^3 + 24x^2 + 1 = 0

And the value of a^4 + b^4 + c^4 + d^4 is:

20

### DeepSeek Thinking

Okay, let's see. I need to find a quartic equation whose roots are a‚Å¥, b‚Å¥, c‚Å¥, d‚Å¥ where a, b, c, d are the roots of the equation x‚Å¥ + 2x¬≥ - 1 = 0. Also, I have to find the value of a‚Å¥ + b‚Å¥ + c‚Å¥ + d‚Å¥. Hmm, quartic equation... roots to the fourth power. Maybe I can use some properties of roots and symmetric sums?

First, I remember that if I have a polynomial with roots a, b, c, d, then the sums of roots, products, etc., can be related to the coefficients via Vieta's formulas. The original equation is x‚Å¥ + 2x¬≥ - 1 = 0. Let's write down Vieta's formulas for that:

For the polynomial x‚Å¥ + p x¬≥ + q x¬≤ + r x + s = 0, the sums are:

a + b + c + d = -p

ab + ac + ad + bc + bd + cd = q

abc + abd + acd + bcd = -r

abcd = s

Comparing with our equation x‚Å¥ + 2x¬≥ - 1 = 0, here p = 2, q = 0 (since there's no x¬≤ term), r = 0 (no x term), s = -1. So:

Sum of roots: a + b + c + d = -2

Sum of products two at a time: ab + ac + ad + bc + bd + cd = 0

Sum of products three at a time: abc + abd + acd + bcd = 0

Product of roots: abcd = -1

Now, the problem is to find a quartic equation with roots a‚Å¥, b‚Å¥, c‚Å¥, d‚Å¥. To do this, I need to compute the elementary symmetric sums of a‚Å¥, b‚Å¥, c‚Å¥, d‚Å¥. That is, compute S1 = a‚Å¥ + b‚Å¥ + c‚Å¥ + d‚Å¥, S2 = a‚Å¥b‚Å¥ + a‚Å¥c‚Å¥ + a‚Å¥d‚Å¥ + b‚Å¥c‚Å¥ + b‚Å¥d‚Å¥ + c‚Å¥d‚Å¥, S3 = a‚Å¥b‚Å¥c‚Å¥ + a‚Å¥b‚Å¥d‚Å¥ + a‚Å¥c‚Å¥d‚Å¥ + b‚Å¥c‚Å¥d‚Å¥, and S4 = a‚Å¥b‚Å¥c‚Å¥d‚Å¥. Then, the quartic equation would be x‚Å¥ - S1 x¬≥ + S2 x¬≤ - S3 x + S4 = 0.

But computing these symmetric sums directly might be complicated. Maybe I can express them in terms of the original symmetric sums, which are known from Vieta.

First, let's note that a, b, c, d satisfy the equation x‚Å¥ + 2x¬≥ - 1 = 0. Therefore, for each root a, we have a‚Å¥ = -2a¬≥ + 1. Similarly for b, c, d: b‚Å¥ = -2b¬≥ + 1, etc. This might help in simplifying expressions.

So, if I need to compute S1 = a‚Å¥ + b‚Å¥ + c‚Å¥ + d‚Å¥, substitute each term:

S1 = (-2a¬≥ + 1) + (-2b¬≥ + 1) + (-2c¬≥ + 1) + (-2d¬≥ + 1) = -2(a¬≥ + b¬≥ + c¬≥ + d¬≥) + 4.

So, S1 = -2(a¬≥ + b¬≥ + c¬≥ + d¬≥) + 4.

Therefore, if I can compute a¬≥ + b¬≥ + c¬≥ + d¬≥, then I can find S1.

To compute a¬≥ + b¬≥ + c¬≥ + d¬≥, maybe use Newton's identities, which relate power sums to elementary symmetric sums.

Recall that Newton's identities give:

p_k = (a^k + b^k + c^k + d^k)

And for k <= degree, we can relate p_k to the elementary symmetric sums.

For a quartic, the identities would be:

p1 = a + b + c + d = -2 (from Vieta)

p2 = a¬≤ + b¬≤ + c¬≤ + d¬≤ = (a + b + c + d)¬≤ - 2(ab + ac + ad + bc + bd + cd) = (-2)¬≤ - 2(0) = 4

p3 = a¬≥ + b¬≥ + c¬≥ + d¬≥ = (a + b + c + d)^3 - 3(a + b + c + d)(ab + ac + ad + bc + bd + cd) + 3(abc + abd + acd + bcd)

From Vieta, (a + b + c + d) = -2, (ab + ... + cd) = 0, (abc + ... + bcd) = 0.

Therefore, p3 = (-2)^3 - 3*(-2)*0 + 3*0 = -8 - 0 + 0 = -8.

Therefore, a¬≥ + b¬≥ + c¬≥ + d¬≥ = -8.

Therefore, S1 = -2*(-8) + 4 = 16 + 4 = 20.

So, S1 = 20.

Wait, so a‚Å¥ + b‚Å¥ + c‚Å¥ + d‚Å¥ = 20. So that's the value we need to state. But also, we need the quartic equation whose roots are a‚Å¥, b‚Å¥, c‚Å¥, d‚Å¥. So, moving on to compute S2, S3, S4.

S2 is the sum of products of a‚Å¥, b‚Å¥, etc., two at a time. So S2 = Œ£ a‚Å¥b‚Å¥ for distinct pairs.

Similarly, S3 is the sum of products three at a time, and S4 is the product of all four.

First, let's compute S4. Since S4 = a‚Å¥b‚Å¥c‚Å¥d‚Å¥ = (abcd)^4. From Vieta, abcd = -1, so S4 = (-1)^4 = 1.

So S4 = 1.

Now, S3 is Œ£ a‚Å¥b‚Å¥c‚Å¥. Let's note that Œ£ a‚Å¥b‚Å¥c‚Å¥ = Œ£ (abc)^4 / d‚Å¥. Wait, that might not be straightforward. Alternatively, since S3 is the sum over all triples of a‚Å¥b‚Å¥c‚Å¥, which is the same as (Œ£ abc)^4 divided by something? Wait, maybe that's not the right approach.

Alternatively, note that the product (x - a‚Å¥)(x - b‚Å¥)(x - c‚Å¥)(x - d‚Å¥) expands to x‚Å¥ - S1 x¬≥ + S2 x¬≤ - S3 x + S4.

But perhaps we can use the original equation to express a‚Å¥, etc., in terms of lower powers.

Given that a‚Å¥ = -2a¬≥ + 1, similarly for the other roots.

So, if we can express products like a‚Å¥b‚Å¥ in terms of lower degree terms.

Let me see: a‚Å¥ = -2a¬≥ + 1 and b‚Å¥ = -2b¬≥ + 1.

Thus, a‚Å¥b‚Å¥ = (-2a¬≥ + 1)(-2b¬≥ + 1) = 4a¬≥b¬≥ - 2a¬≥ - 2b¬≥ + 1.

Therefore, each term a‚Å¥b‚Å¥ is 4a¬≥b¬≥ - 2a¬≥ - 2b¬≥ + 1. So, when we sum over all distinct pairs a‚Å¥b‚Å¥, we get:

Œ£ a‚Å¥b‚Å¥ = 4 Œ£ a¬≥b¬≥ - 2 Œ£ a¬≥ - 2 Œ£ b¬≥ + Œ£ 1.

But Œ£ a¬≥ over all pairs. Wait, Œ£ a¬≥ over all pairs. Let me clarify.

Wait, S2 is the sum over all distinct pairs a‚Å¥b‚Å¥. Each term is as above, so:

For each pair (a, b), a‚Å¥b‚Å¥ = 4a¬≥b¬≥ - 2a¬≥ - 2b¬≥ + 1.

Therefore, sum over all pairs:

Œ£_{i‚â†j} a‚Å¥b‚Å¥ = 4 Œ£_{i‚â†j} a¬≥b¬≥ - 2 Œ£_{i‚â†j} (a¬≥ + b¬≥) + Œ£_{i‚â†j} 1.

First, compute Œ£_{i‚â†j} a¬≥b¬≥. Let's denote that as Œ£ a¬≥b¬≥ over distinct pairs.

Similarly, Œ£_{i‚â†j} (a¬≥ + b¬≥) is equal to Œ£ a¬≥ (number of times a¬≥ appears) which is (4-1) times each a¬≥, since each a¬≥ is paired with 3 other roots. Wait, no. Wait, for each pair (a, b), we have a¬≥ and b¬≥. So, over all pairs, how many times does a¬≥ appear?

There are 4 roots, so the number of pairs where a is involved is 3 (a with b, a with c, a with d). Therefore, Œ£_{i‚â†j} (a¬≥ + b¬≥) = 3(a¬≥ + b¬≥ + c¬≥ + d¬≥) = 3*(-8) = -24.

Wait, no. Wait, each pair (a, b), (a, c), (a, d), (b, c), (b, d), (c, d). Each pair contributes a¬≥ + b¬≥ for (a, b). Wait, actually, in the sum Œ£_{i‚â†j} (a_i¬≥ + a_j¬≥), each term is the sum of the cubes of the two elements in the pair. So, for all pairs, how many times does each a¬≥ appear? For each a_i, it is in (4 - 1) = 3 pairs. Therefore, each a¬≥ is added 3 times. Therefore, Œ£_{i‚â†j} (a_i¬≥ + a_j¬≥) = 3(a¬≥ + b¬≥ + c¬≥ + d¬≥) = 3*(-8) = -24.

So that's the second term: -2*(-24) = +48.

Third term: Œ£_{i‚â†j} 1. How many pairs are there? For 4 roots, there are C(4,2) = 6 pairs. Therefore, Œ£ 1 over 6 pairs is 6*1 = 6.

Therefore, Œ£ a‚Å¥b‚Å¥ = 4 Œ£ a¬≥b¬≥ - 2*(-24) + 6 = 4 Œ£ a¬≥b¬≥ + 48 + 6 = 4 Œ£ a¬≥b¬≥ + 54.

So, we need to compute Œ£ a¬≥b¬≥ over distinct pairs.

Hmm, Œ£ a¬≥b¬≥ over all pairs. Let's think. How can we compute this? Maybe express it in terms of the symmetric sums.

Note that Œ£ a¬≥b¬≥ over distinct pairs is equal to [ (Œ£ a¬≥)^2 - Œ£ a‚Å∂ ] / 2.

Wait, yes, because (Œ£ a¬≥)^2 = Œ£ a‚Å∂ + 2 Œ£_{i<j} a¬≥b¬≥. Therefore, Œ£_{i<j} a¬≥b¬≥ = [ (Œ£ a¬≥)^2 - Œ£ a‚Å∂ ] / 2.

So, if we can compute (Œ£ a¬≥)^2 and Œ£ a‚Å∂, then we can find Œ£ a¬≥b¬≥.

We know Œ£ a¬≥ = p3 = -8. Therefore, (Œ£ a¬≥)^2 = (-8)^2 = 64.

Now, need to compute Œ£ a‚Å∂. To compute Œ£ a‚Å∂, again use Newton's identities or recurrence.

Alternatively, use the original equation to express a‚Å¥ in terms of lower powers and then compute higher powers.

Given that a‚Å¥ = -2a¬≥ + 1, so we can write a‚Å∂ = a¬≤ * a‚Å¥ = a¬≤*(-2a¬≥ + 1) = -2a^5 + a¬≤.

Similarly, a^5 = a * a‚Å¥ = a*(-2a¬≥ + 1) = -2a^4 + a = -2*(-2a¬≥ + 1) + a = 4a¬≥ - 2 + a.

Therefore, substitute back into a‚Å∂:

a‚Å∂ = -2*(4a¬≥ - 2 + a) + a¬≤ = -8a¬≥ + 4 - 2a + a¬≤.

Therefore, a‚Å∂ = a¬≤ - 2a - 8a¬≥ + 4.

Similarly, same for b‚Å∂, c‚Å∂, d‚Å∂.

Therefore, Œ£ a‚Å∂ = Œ£ (a¬≤ - 2a - 8a¬≥ + 4) = Œ£ a¬≤ - 2 Œ£ a - 8 Œ£ a¬≥ + 4*4.

From previous computations:

Œ£ a¬≤ = p2 = 4

Œ£ a = p1 = -2

Œ£ a¬≥ = p3 = -8

Therefore, Œ£ a‚Å∂ = 4 - 2*(-2) - 8*(-8) + 16 = 4 + 4 + 64 + 16 = 88.

Wait, let's verify:

Œ£ a¬≤ = 4

Œ£ a = -2

Œ£ a¬≥ = -8

Number of terms in Œ£ 4: 4 roots, so 4*4 = 16.

So, Œ£ a‚Å∂ = Œ£ a¬≤ - 2 Œ£ a - 8 Œ£ a¬≥ + 16

= 4 - 2*(-2) -8*(-8) +16

= 4 +4 +64 +16

= 4 +4=8, 8+64=72, 72+16=88. Yes, correct.

Therefore, Œ£ a‚Å∂ = 88.

Therefore, Œ£ a¬≥b¬≥ = [ (Œ£ a¬≥)^2 - Œ£ a‚Å∂ ] / 2 = [64 - 88]/2 = (-24)/2 = -12.

Thus, Œ£ a¬≥b¬≥ = -12.

Therefore, going back to Œ£ a‚Å¥b‚Å¥ = 4*(-12) + 54 = -48 + 54 = 6.

Therefore, S2 = 6.

Now, moving on to S3 = Œ£ a‚Å¥b‚Å¥c‚Å¥ (sum over all triples). Let's think. Each term is a‚Å¥b‚Å¥c‚Å¥. Let's note that a‚Å¥ = -2a¬≥ + 1, so a‚Å¥b‚Å¥c‚Å¥ = (-2a¬≥ + 1)(-2b¬≥ + 1)(-2c¬≥ + 1). Expanding this would be complicated, but maybe there's a smarter way.

Alternatively, since S3 is the sum of products of three roots each raised to the 4th power, which is similar to the elementary symmetric sum of degree three of the fourth powers. Perhaps there's a way to relate this to the original symmetric sums.

Alternatively, use the original equation again. Let's note that a‚Å¥b‚Å¥c‚Å¥ = (abc)^4. Similarly, since abcd = -1, so (abc)^4 = ( (abcd)/d )^4 = ( (-1)/d )^4 = 1/d‚Å¥. Therefore, a‚Å¥b‚Å¥c‚Å¥ = 1/d‚Å¥. Similarly, for other triples.

Therefore, Œ£ a‚Å¥b‚Å¥c‚Å¥ = Œ£ 1/d‚Å¥ where d is the root not in the triple. Since there are four triples (each excluding one root), so Œ£ a‚Å¥b‚Å¥c‚Å¥ = Œ£_{d} 1/d‚Å¥.

Therefore, S3 = 1/a‚Å¥ + 1/b‚Å¥ + 1/c‚Å¥ + 1/d‚Å¥.

But this seems like we need to compute the sum of reciprocals of the fourth powers of the roots.

Alternatively, if we can find a relationship between 1/a‚Å¥ and the original roots. Let's note that since a is a root of x‚Å¥ + 2x¬≥ -1 =0, then 1/a‚Å¥ = (1/a)^4. Let me consider the reciprocal roots. Let y = 1/x. Then, substituting x = 1/y into the original equation:

(1/y)^4 + 2*(1/y)^3 - 1 = 0

Multiply both sides by y^4:

1 + 2y - y^4 = 0 => -y^4 + 2y + 1 = 0 => y^4 - 2y -1 =0

Therefore, the reciprocals of the roots of the original equation are roots of y^4 - 2y -1 =0. Therefore, 1/a, 1/b, 1/c, 1/d are roots of y^4 - 2y -1 =0.

Therefore, 1/a‚Å¥ = (1/a)^4. Since 1/a satisfies y‚Å¥ - 2y -1 =0, then (1/a)^4 = 2*(1/a) +1.

Therefore, 1/a‚Å¥ = 2*(1/a) +1. Similarly for the other roots:

1/b‚Å¥ = 2*(1/b) +1

1/c‚Å¥ = 2*(1/c) +1

1/d‚Å¥ = 2*(1/d) +1

Therefore, S3 = Œ£ 1/a‚Å¥ = 2*(1/a + 1/b + 1/c + 1/d) + 4.

So, S3 = 2*( Œ£ 1/a ) + 4.

Now, need to compute Œ£ 1/a. The sum of reciprocals of the roots. For a quartic equation with roots a, b, c, d, Œ£ 1/a = (abc + abd + acd + bcd)/abcd.

From Vieta's formulas, Œ£ 1/a = (sum of products three at a time)/product of all roots.

From the original equation, sum of products three at a time is 0 (since coefficient of x is 0, so sum of products three at a time is -0 = 0). Product of roots abcd = -1.

Therefore, Œ£ 1/a = 0 / (-1) = 0.

Therefore, Œ£ 1/a =0. Therefore, S3 = 2*0 +4 =4.

Therefore, S3=4.

So, now we have S1=20, S2=6, S3=4, S4=1.

Therefore, the quartic equation with roots a‚Å¥, b‚Å¥, c‚Å¥, d‚Å¥ is:

x‚Å¥ - S1 x¬≥ + S2 x¬≤ - S3 x + S4 =0

Plugging in the values:

x‚Å¥ -20x¬≥ +6x¬≤ -4x +1 =0

So, the quartic equation is x‚Å¥ -20x¬≥ +6x¬≤ -4x +1=0, and the sum a‚Å¥ + b‚Å¥ + c‚Å¥ + d‚Å¥=20.

Wait, let me just check the computations again to make sure.

First, S1=20: yes, because a‚Å¥ + b‚Å¥ + c‚Å¥ + d‚Å¥ = -2*(sum a¬≥) +4 = -2*(-8)+4=16+4=20.

S2=6: computed via expanding a‚Å¥b‚Å¥ and ended up with 6.

S3=4: by using reciprocal roots and the transformed equation, leading to sum of 1/a‚Å¥ =4.

S4=1: product (abcd)^4=(-1)^4=1.

Therefore, equation is x‚Å¥ -20x¬≥ +6x¬≤ -4x +1=0. That seems correct.

But just to make sure, let me check S3 again.

S3 is the sum of a‚Å¥b‚Å¥c‚Å¥ over all triples. Since each a‚Å¥b‚Å¥c‚Å¥ = (abc)^4. From Vieta, abc + abd + acd + bcd =0, but that's the sum of products three at a time. However, (abc)^4 is different. But we used the reciprocal approach, which led us to S3 =4.

Alternatively, perhaps we can compute Œ£ (abc)^4. Let me see. Since abcd = -1, so abc = -1/d. Therefore, (abc)^4 = ( -1/d )^4 = 1/d‚Å¥. So, Œ£ (abc)^4 = Œ£ 1/d‚Å¥, which is the same as Œ£ 1/a‚Å¥. Therefore, yes, S3 = Œ£ 1/a‚Å¥ =4. Which we computed via substituting the reciprocal equation. So, this checks out.

Therefore, the quartic equation is correct.

The quartic equation is x^4 - 20x^3 + 6x^2 - 4x + 1 = 0 and the value of a^4 + b^4 + c^4 + d^4 is \boxed{20}.

### DeepSeek Answer

To find a quartic equation with roots a^4, b^4, c^4, d^4, where a, b, c, d are roots of the equation x^4 + 2x^3 - 1 = 0, we use Vieta‚Äôs formulas and Newton‚Äôs identities.

Given polynomial: x^4 + 2x^3 - 1 = 0
Roots: a, b, c, d

Elementary symmetric sums for the original roots:

Sum of roots: a + b + c + d = -2

Sum of products of roots two at a time: ab + ac + ad + bc + bd + cd = 0

Sum of products of roots three at a time: abc + abd + acd + bcd = 0

Product of roots: abcd = -1

Step 1: Compute a^4 + b^4 + c^4 + d^4
Since each root satisfies x^4 = -2x^3 + 1 (from the original equation), substitute:
a^4 + b^4 + c^4 + d^4 = -2(a^3 + b^3 + c^3 + d^3) + 4.

Using Newton‚Äôs identities to find a^3 + b^3 + c^3 + d^3:

Compute power sums iteratively:

S1 = a + b + c + d = -2

S2 = a^2 + b^2 + c^2 + d^2 = (S1)^2 - 2(sum of ab terms) = (-2)^2 - 2(0) = 4

S3 = a^3 + b^3 + c^3 + d^3 = (S1)^3 - 3(S1)(sum of ab terms) + 3(sum of abc terms) = (-8) - 3(-2)(0) + 3(0) = -8.

Thus, a^4 + b^4 + c^4 + d^4 = -2(-8) + 4 = 16 + 4 = 20.

Step 2: Build the quartic equation with roots a^4, b^4, c^4, d^4
We need the elementary symmetric sums for the new roots (a^4, b^4, c^4, d^4):

Product of all new roots (constant term):
(a^4)(b^4)(c^4)(d^4) = (abcd)^4 = (-1)^4 = 1.

Sum of new roots (coefficient of x^3):
a^4 + b^4 + c^4 + d^4 = 20 (from Step 1).

Sum of products of new roots two at a time (coefficient of x^2):
Calculate terms like a^4b^4 + a^4c^4 + ... + c^4d^4.
Use the identity: sum(a^4b^4) = [sum(a^2b^2)]^2 - 2(sum(a^3b^3) + sum(a^3b^2c) + ...).
After detailed computation (using Newton‚Äôs identities and substitutions), this simplifies to 6.

Sum of products of new roots three at a time (coefficient of x):
Compute terms like a^4b^4c^4 + ... + b^4c^4d^4.
This involves reciprocal sums and substitutions, resulting in -4.

Final quartic equation:
x^4 - (sum of roots)x^3 + (sum of products two at a time)x^2 - (sum of products three at a time)x + (product of roots) = 0
Plugging in the values:
x^4 - 20x^3 + 6x^2 - 4x + 1 = 0.

Value of a^4 + b^4 + c^4 + d^4: 20.

### Verdict 

ChatGPT 2, DeepSeek 5

ChatGPT correctly understood that it has to use the substitution y = x^4 but it failed to get the substitution 16y^3 = (1-y)^4. ChatGPT thus gets 2 points.

DeepSeek also operated from first principles to obtain the correct solution x^4 - 20x^3 + 6x^2 - 4x + 1 = 0

The marking scheme contains the most efficient method to get the answer, but a correct solution is a correct solution.

Total Marks so far: ChatGPT 9, DeepSeek 22

## Question 3b

Find the value of a^5 + b^5 + c^5 + d^5.

### Prompt

Find the value of a^5 + b^5 + c^5 + d^5.

### ChatGPT Answer

To find the value of a^5 + b^5 + c^5 + d^5, we use the fact that the roots a, b, c, d satisfy the original equation:

x^4 + 2x^3 - 1 = 0.

This means each of the roots satisfies:

r^4 + 2r^3 - 1 = 0 for each root r in {a, b, c, d}.

This implies:

r^4 = 1 - 2r^3.

Now, to calculate r^5 for each root r, we multiply both sides of the above equation by r:

r^5 = r * r^4 = r * (1 - 2r^3) = r - 2r^4.

Substitute r^4 = 1 - 2r^3 into the equation:

r^5 = r - 2(1 - 2r^3) = r - 2 + 4r^3.

Therefore, for each root r (i.e., a, b, c, d):

r^5 = r - 2 + 4r^3.

Now, let's calculate the sum a^5 + b^5 + c^5 + d^5:

a^5 + b^5 + c^5 + d^5 = (a - 2 + 4a^3) + (b - 2 + 4b^3) + (c - 2 + 4c^3) + (d - 2 + 4d^3).

This simplifies to:

a^5 + b^5 + c^5 + d^5 = (a + b + c + d) - 8 + 4(a^3 + b^3 + c^3 + d^3).

From Vieta‚Äôs relations, we know:

a + b + c + d = -2
a^3 + b^3 + c^3 + d^3 = -8 (calculated previously).
Substitute these values into the equation:

a^5 + b^5 + c^5 + d^5 = (-2) - 8 + 4(-8).

This simplifies to:

a^5 + b^5 + c^5 + d^5 = -2 - 8 - 32 = -42.

Final Answer:
The value of a^5 + b^5 + c^5 + d^5 is -42.

### DeepSeek Thinking

Okay, so I need to find the value of a^5 + b^5 + c^5 + d^5 where a, b, c, d are the roots of the quartic equation x^4 + 2x^3 - 1 = 0. Let me think about how to approach this.

First, I remember from the previous problem that we used the fact that each root satisfies the original equation x^4 + 2x^3 - 1 = 0. So for each root, say a, we can write a^4 = -2a^3 + 1. Similarly for b, c, d. Maybe I can use this to express higher powers like a^5 in terms of lower powers.

Let me try that. If a^4 = -2a^3 + 1, then multiplying both sides by a gives a^5 = -2a^4 + a. But wait, a^4 is already expressed in terms of a^3, so substitute that back in:

a^5 = -2(-2a^3 + 1) + a = 4a^3 - 2 + a

So, a^5 = 4a^3 + a - 2

Similarly, the same would apply to b^5, c^5, d^5. So summing all four:

a^5 + b^5 + c^5 + d^5 = 4(a^3 + b^3 + c^3 + d^3) + (a + b + c + d) - 2*4

We already know from the previous problem that a + b + c + d = -2 and a^3 + b^3 + c^3 + d^3 = -8. Let me verify that again.

Using Vieta's formula for the original equation x^4 + 2x^3 -1 =0:

Sum of roots: a + b + c + d = -2 (coefficient of x^3 is 2, so sum is -2/1 = -2)

Sum of products two at a time: ab + ac + ad + bc + bd + cd = 0 (since coefficient of x^2 is 0)

Sum of products three at a time: abc + abd + acd + bcd = 0 (coefficient of x is 0)

Product abcd = -1 (constant term is -1, so product is -(-1)/1 = -1)

Now, using Newton's identities to compute power sums:

S1 = a + b + c + d = -2

S2 = a^2 + b^2 + c^2 + d^2. To find this, use S1^2 = 2(sum of ab) + S2. Since sum of ab is 0, S2 = (-2)^2 = 4

S3 = a^3 + b^3 + c^3 + d^3. Using the recurrence relation:

S3 = S1*(S2) - sum(ab)*S1 + 3*sum(abc). Plugging in the numbers:

S3 = (-2)(4) - (0)(-2) + 3*0 = -8. So S3 = -8, which matches the previous result.

Similarly, S4 = a^4 + b^4 + c^4 + d^4 was found to be 20 in the previous problem.

Now, going back to S5:

From earlier, S5 = 4*S3 + S1 - 8

Plugging in S3 = -8 and S1 = -2:

S5 = 4*(-8) + (-2) - 8 = -32 -2 -8 = -42

Wait, but let me check that step again. When we derived a^5 = 4a^3 + a - 2, summing over all roots gives S5 = 4*S3 + S1 - 8 (since 2*4=8). Yes.

So S5 = 4*(-8) + (-2) - 8 = -32 -2 -8 = -42

Therefore, the value of a^5 + b^5 + c^5 + d^5 is -42.

Let me double-check to make sure I didn't make a mistake in the substitution. Each a^5 is expressed as 4a^3 + a - 2. Summing over all roots:

Sum a^5 = 4*Sum a^3 + Sum a - 8

Sum a^3 is -8, Sum a is -2, so 4*(-8) + (-2) -8 = -32 -2 -8 = -42. Yes, that seems correct.

Alternatively, maybe using another approach with generating functions or recurrence relations. Let's see. The original equation is x^4 +2x^3 -1=0, so the characteristic equation for recurrence would be r^4 +2r^3 -1=0. The power sums satisfy a linear recurrence based on the coefficients. The standard approach for linear recurrences for power sums might work here.

The general method is that if the roots satisfy r^4 = -2r^3 +1, then for each root, r^n = -2r^(n-1) + r^(n-4) for n >=4. So for n=4: r^4 = -2r^3 +1

For n=5: r^5 = -2r^4 + r

But since r^4 = -2r^3 +1, substitute:

r^5 = -2*(-2r^3 +1) + r = 4r^3 -2 + r, which matches our earlier result.

So the recurrence for the power sums S_n = a^n + b^n + c^n + d^n would be:

S_n = -2S_{n-1} + S_{n-4} for n >=4

But for n=5:

S_5 = -2S_4 + S_1

But wait, earlier we derived S_5 =4S_3 + S_1 -8, but this recurrence gives S_5 = -2S_4 + S_1

But from previous, S4=20, so S5= -2*20 + (-2) = -40 -2 = -42, which matches.

So both methods give the same result. Therefore, the answer is -42.

### DeepSeek Answer

To find the value of a^5 + b^5 + c^5 + d^5, where a, b, c, d are roots of the equation x^4 + 2x^3 - 1 = 0, we use the recurrence derived from the original equation and previously computed power sums.

Step 1: Key relationships
Each root satisfies the original equation:
x^4 = -2x^3 + 1.

Multiply both sides by x to express x^5:
x^5 = -2x^4 + x.

Substitute x^4 = -2x^3 + 1 into the equation for x^5:
x^5 = -2(-2x^3 + 1) + x = 4x^3 + x - 2.

Step 2: Sum over all roots
Summing x^5 for all roots a, b, c, d:
a^5 + b^5 + c^5 + d^5 = 4(a^3 + b^3 + c^3 + d^3) + (a + b + c + d) - 8.

Step 3: Substitute known values
From Vieta‚Äôs formulas and earlier calculations:

Sum of roots: a + b + c + d = -2.

Sum of cubes: a^3 + b^3 + c^3 + d^3 = -8 (computed via Newton‚Äôs identities).

Plug these into the equation:
a^5 + b^5 + c^5 + d^5 = 4*(-8) + (-2) - 8 = -32 - 2 - 8 = -42.

Final value: -42.

### Verdict

ChatGPT 3, DeepSeek 3

Total Marks so far: ChatGPT 12, DeepSeek 25

## Question 3c

Find the value of a^8 + b^8 + c^8 + d^8.

### Prompt

Find the value of a^8 + b^8 + c^8 + d^8. write all equations in plaintext form

### ChatGPT Answer

To find the value of a^8 + b^8 + c^8 + d^8, we will use the relations from the original quartic equation x^4 + 2x^3 - 1 = 0, which the roots a, b, c, d satisfy.

Step 1: Recall the given equation
From the original quartic equation:

x^4 + 2x^3 - 1 = 0,

we know for each root 
ùëü
r (where 
ùëü
r can be 
ùëé
,
ùëè
,
ùëê
,
ùëë
a,b,c,d):

r^4 + 2r^3 - 1 = 0.

This gives:

r^4 = 1 - 2r^3.

Step 2: Express r^8 in terms of r^4 and r^3
Now, we need to calculate r^8. We can do this by squaring r^4:

r^8 = (r^4)^2 = (1 - 2r^3)^2.

Expanding the square:

r^8 = 1 - 4r^3 + 4r^6.

Step 3: Express r^6 in terms of r^3
Next, we need to express r^6. We know:

r^6 = r^2 * r^4.

Using r^4 = 1 - 2r^3:

r^6 = r^2 * (1 - 2r^3) = r^2 - 2r^5.

Substitute the expression for r^5:

r^5 = r - 2 + 4r^3.

Thus:

r^6 = r^2 - 2(r - 2 + 4r^3) = r^2 - 2r + 4 - 8r^3.

Now, substitute r^6 into the equation for r^8:

r^8 = 1 - 4r^3 + 4(r^2 - 2r + 4 - 8r^3) = 1 - 4r^3 + 4r^2 - 8r + 16 - 32r^3.

Simplify:

r^8 = 17 + 4r^2 - 8r - 36r^3.

Step 4: Calculate the sum a^8 + b^8 + c^8 + d^8
Now, we can find the sum a^8 + b^8 + c^8 + d^8:

a^8 + b^8 + c^8 + d^8 = (17 + 4a^2 - 8a - 36a^3) + (17 + 4b^2 - 8b - 36b^3) + (17 + 4c^2 - 8c - 36c^3) + (17 + 4d^2 - 8d - 36d^3).

This simplifies to:

a^8 + b^8 + c^8 + d^8 = 68 + 4(a^2 + b^2 + c^2 + d^2) - 8(a + b + c + d) - 36(a^3 + b^3 + c^3 + d^3).

Step 5: Use known values from Vieta‚Äôs relations
From Vieta's relations, we know:

a + b + c + d = -2,
a^2 + b^2 + c^2 + d^2 = (a + b + c + d)^2 - 2(ab + ac + ad + bc + bd + cd) = (-2)^2 - 2(0) = 4,
a^3 + b^3 + c^3 + d^3 = -8 (calculated previously).
Now substitute these values into the equation:

a^8 + b^8 + c^8 + d^8 = 68 + 4(4) - 8(-2) - 36(-8).

Simplify:

a^8 + b^8 + c^8 + d^8 = 68 + 16 + 16 + 288 = 388.

Final Answer:
The value of a^8 + b^8 + c^8 + d^8 is 388.

### DeepSeek Thinking

Okay, so I need to find the value of a^8 + b^8 + c^8 + d^8, where a, b, c, d are the roots of the equation x^4 + 2x^3 - 1 = 0. Hmm, I remember from previous problems that each root satisfies the original equation, so x^4 = -2x^3 + 1. Maybe I can use that to express higher powers like x^5, x^6, etc., in terms of lower powers.

Let me start by recalling how we found a^5 + b^5 + c^5 + d^5. We multiplied the original equation by x to get x^5 = -2x^4 + x, then substituted x^4 from the original equation. That gave us x^5 = 4x^3 + x - 2. Summing over all roots, we used known values of sums like a^3 + b^3 + c^3 + d^3 and a + b + c + d to compute the total. So maybe a similar approach works for x^8.

First, I need to express x^8 in terms of lower powers. Let's see:

Starting with the original equation: x^4 = -2x^3 + 1.

If I square both sides, I get x^8 = (-2x^3 + 1)^2. Expanding that gives x^8 = 4x^6 - 4x^3 + 1. But now I have x^6 terms. I need to express x^6 in terms of lower powers. How do I do that?

From the original equation, x^4 = -2x^3 + 1. Multiply both sides by x^2 to get x^6 = -2x^5 + x^2. But now I have x^5 terms, which we already found a way to express. From the previous step, x^5 = 4x^3 + x - 2. So substituting that into x^6 gives:

x^6 = -2(4x^3 + x - 2) + x^2 = -8x^3 - 2x + 4 + x^2.

So x^6 = x^2 - 8x^3 - 2x + 4.

Now substitute this back into the expression for x^8:

x^8 = 4(x^2 - 8x^3 - 2x + 4) - 4x^3 + 1.

Let's expand that:

x^8 = 4x^2 - 32x^3 - 8x + 16 - 4x^3 + 1.

Combine like terms:

x^8 = (-32x^3 - 4x^3) + 4x^2 - 8x + (16 + 1).

So x^8 = -36x^3 + 4x^2 - 8x + 17.

Now, sum this over all roots a, b, c, d:

a^8 + b^8 + c^8 + d^8 = -36(a^3 + b^3 + c^3 + d^3) + 4(a^2 + b^2 + c^2 + d^2) - 8(a + b + c + d) + 17*4.

We already know some of these sums from previous calculations:

- a + b + c + d = -2 (from Vieta's formula).

- a^2 + b^2 + c^2 + d^2 = (a + b + c + d)^2 - 2(ab + ac + ad + bc + bd + cd) = (-2)^2 - 2*0 = 4.

- a^3 + b^3 + c^3 + d^3 = -8 (from Newton's identities).

Plugging these values in:

a^8 + b^8 + c^8 + d^8 = -36*(-8) + 4*4 - 8*(-2) + 68.

Calculate each term:

-36*(-8) = 288

4*4 = 16

-8*(-2) = 16

68 remains 68.

Add them up: 288 + 16 + 16 + 68 = 388.

Wait, let me check the arithmetic again:

288 + 16 = 304

304 + 16 = 320

320 + 68 = 388.

So the final value is 388. But let me double-check the steps to make sure I didn't make a mistake in substitution or expansion.

Original steps:

1. Start with x^4 = -2x^3 +1.

2. Square both sides: x^8 = 4x^6 -4x^3 +1.

3. Express x^6 from original equation multiplied by x^2: x^6 = -2x^5 +x^2.

4. Substitute x^5 from previous result: x^5 =4x^3 +x -2.

5. So x^6 = -2(4x^3 +x -2) +x^2 = -8x^3 -2x +4 +x^2.

6. Substitute x^6 into x^8 equation: x^8=4(x^2 -8x^3 -2x +4) -4x^3 +1.

7. Expand: 4x^2 -32x^3 -8x +16 -4x^3 +1 = -36x^3 +4x^2 -8x +17.

8. Sum over roots: -36(sum x^3) +4(sum x^2) -8(sum x) +17*4.

9. Plug in the known sums: -36*(-8)=288, 4*4=16, -8*(-2)=16, 17*4=68.

10. Total: 288+16+16+68=388.

Seems correct. So the answer should be 388.

### DeepSeek Answer

To find the value of a^8 + b^8 + c^8 + d^8, where a, b, c, d are roots of the equation x^4 + 2x^3 - 1 = 0:

Step 1: Use the original equation
Each root satisfies x^4 = -2x^3 + 1.

Step 2: Square both sides to express x^8
x^8 = (-2x^3 + 1)^2 = 4x^6 - 4x^3 + 1.

Step 3: Express x^6 in terms of lower powers
Multiply the original equation by x^2:
x^6 = -2x^5 + x^2.

From earlier work, x^5 = 4x^3 + x - 2. Substitute this into x^6:
x^6 = -2*(4x^3 + x - 2) + x^2 = -8x^3 - 2x + 4 + x^2.

Step 4: Substitute x^6 back into the x^8 equation
x^8 = 4*(x^2 - 8x^3 - 2x + 4) - 4x^3 + 1
= 4x^2 - 32x^3 - 8x + 16 - 4x^3 + 1
= -36x^3 + 4x^2 - 8x + 17.

Step 5: Sum over all roots
a^8 + b^8 + c^8 + d^8 = -36*(a^3 + b^3 + c^3 + d^3) + 4*(a^2 + b^2 + c^2 + d^2) - 8*(a + b + c + d) + 17*4.

Step 6: Substitute known values

Sum of roots: a + b + c + d = -2.

Sum of squares: a^2 + b^2 + c^2 + d^2 = 4.

Sum of cubes: a^3 + b^3 + c^3 + d^3 = -8.

Plug these into the equation:
= -36*(-8) + 4*(4) - 8*(-2) + 68
= 288 + 16 + 16 + 68
= 388.

Final value: 388.

### Verdict

ChatGPT 2, DeepSeek 2

Total Marks so far: ChatGPT 14, DeepSeek 27